cava/Cava/Acorn/Circuit.v
@@ -30,20 +30,18 @@ Require Import Cava.Acorn.Combinators.
 Section WithCava.
   Context `{semantics:Cava}.
 
-  (* TODO: change loop here to a loop with enable *)
-  (* TODO: maybe make loop have separate in/out types to reduce state info *)
   Inductive Circuit : Type -> Type -> Type :=
   | Comb : forall {i o}, (i -> cava o) -> Circuit i o
   | Compose : forall {i t o}, Circuit i t -> Circuit t o -> Circuit i o
   | First : forall {i o t}, Circuit i o -> Circuit (i * t) (o * t)
   | Second : forall {i o t}, Circuit i o -> Circuit (t * i) (t * o)
   | LoopInitCE :
-      forall {i o : Type} {s : SignalType} (en : signal Bit) (resetval : signal s),
+      forall {i o : Type} {s : SignalType} (resetval : signal s),
         Circuit (i * signal s) (o * signal s) ->
-        Circuit i o
+        Circuit (i * signal Bit) o
   | DelayInitCE :
-      forall {t} (en : signal Bit) (resetval : signal t),
-        Circuit (signal t) (signal t)
+      forall {t} (resetval : signal t),
+        Circuit (signal t * signal Bit) (signal t)
   .
 
   (* Internal state of the circuit (register values) *)
@@ -53,8 +51,8 @@ Section WithCava.
     | Compose f g => circuit_state f * circuit_state g
     | First f => circuit_state f
     | Second f => circuit_state f
-    | @LoopInitCE i o s _ _ f => circuit_state f * signal s
-    | @DelayInitCE t _ _ => signal t
+    | @LoopInitCE i o s _ f => circuit_state f * signal s
+    | @DelayInitCE t _ => signal t
     end.
 
   (* The state of the circuit after a reset *)
@@ -64,67 +62,37 @@ Section WithCava.
     | Compose f g => (reset_state f, reset_state g)
     | First f => reset_state f
     | Second f => reset_state f
-    | LoopInitCE _ resetval f => (reset_state f, resetval)
-    | DelayInitCE _ resetval => resetval
-    end.
-
-  (* Run circuit for a single step *)
-  Fixpoint interp {i o} (c : Circuit i o)
-    : circuit_state c -> i -> cava (o * circuit_state c) :=
-    match c in Circuit i o return circuit_state c -> i
-                                  -> cava (o * circuit_state c) with
-    | Comb f => fun _ i => x <- f i ;; ret (x, tt)
-    | Compose f g =>
-      fun cs input =>
-        '(x, cs1) <- interp f (fst cs) input ;;
-        '(y, cs2) <- interp g (snd cs) x ;;
-        ret (y, (cs1, cs2))
-    | First f =>
-      fun cs input =>
-        '(x, cs') <- interp f cs (fst input) ;;
-        ret (x, snd input, cs')
-    | Second f =>
-      fun cs input =>
-        '(x, cs') <- interp f cs (snd input) ;;
-        ret (fst input, x, cs')
-    | LoopInitCE en _ f =>
-      fun '(cs,st) input =>
-        '(out, st', cs') <- interp f cs (input, st) ;;
-        (* select the updated state only if the loop is enabled *)
-         let new_state := indexAt (unpeel [st;st']) (unpeel [en]) in
-        ret (out, (cs',new_state))
-    | DelayInitCE en _ =>
-      fun st input =>
-        (* select the updated state only if the delay is enabled *)
-        let new_state := indexAt (unpeel [st;input]) (unpeel [en]) in
-        ret (st, new_state)
+    | LoopInitCE resetval f => (reset_state f, resetval)
+    | DelayInitCE resetval => resetval
     end.
 
   (* Loop with no enable; set enable to always be true *)
   Definition LoopInit {i o s} (resetval : signal s)
-    : Circuit (i * signal s) (o * signal s) -> Circuit i o :=
-    LoopInitCE (constant true) resetval.
+             (body : Circuit (i * signal s) (o * signal s))
+    : Circuit i o :=
+    Compose (Comb (fun i => ret (i, constant true))) (LoopInitCE resetval body).
   (* Delay with no enable; set enable to always be true *)
   Definition DelayInit {t} (resetval : signal t)
     : Circuit (signal t) (signal t) :=
-    DelayInitCE (constant true) resetval.
+    Compose (Comb (fun i => ret (i, constant true))) (DelayInitCE resetval).
 
   (* Loop with the default signal as its reset value *)
-  Definition LoopCE {i o s} (en : signal Bit)
-    : Circuit (i * signal s) (o * signal s) -> Circuit i o :=
-    LoopInitCE en defaultSignal.
+  Definition LoopCE {i o s}
+    : Circuit (i * signal s) (o * signal s) -> Circuit (i * signal Bit) o :=
+    LoopInitCE defaultSignal.
   (* Delay with the default signal as its reset value *)
-  Definition DelayCE {t} (en : signal Bit)
-    : Circuit (signal t) (signal t) :=
-    DelayInitCE en defaultSignal.
+  Definition DelayCE {t}
+    : Circuit (signal t * signal Bit) (signal t) :=
+    DelayInitCE defaultSignal.
 
   (* Loop with the default signal as its reset value and no enable *)
   Definition Loop {i o s}
-    : Circuit (i * signal s) (o * signal s) -> Circuit i o :=
-    LoopInitCE (constant true) defaultSignal.
+             (body : Circuit (i * signal s) (o * signal s))
+    : Circuit i o :=
+    Compose (Comb (fun i => ret (i, constant true))) (LoopInitCE defaultSignal body).
   (* Delay with the default signal as its reset value and no enable *)
   Definition Delay {t} : Circuit (signal t) (signal t) :=
-    DelayInitCE (constant true) defaultSignal.
+    Compose (Comb (fun i => ret (i, constant true))) (DelayInitCE defaultSignal).
 End WithCava.
 
 Module Notations.
